riscv_model/spec/bv_ops_nl.dfy
@@ -7,6 +7,19 @@ module bv_ops_nl {
 
     import opened Power2
     import opened DivMod
+    
+    lemma div_bound(x: int, n: nat)
+      requires n > 0
+      ensures x >= 0 ==> 0 <= x/n <= x
+      ensures x < 0 ==> 0 > (x/n) >= x
+    {
+      if x >= 0 {
+        LemmaDivNonincreasingAuto();
+        LemmaDivPosIsPosAuto();
+      } else {
+        assume false;
+      }
+    }
 
     /* signed operations */
     function method int32_rs(x: int32, shift: nat) : int32
